zoo_persistent: Add persistent union-find (puf).

lib/zoo_persistent/puf.ml
@@ -1,0 +1,56 @@
+type descr =
+  | Root of int
+  | Link of element
+
+and element =
+  descr Pstore_2.ref
+
+type t =
+  descr Pstore_2.t
+
+let create =
+  Pstore_2.create
+
+let make t =
+  Pstore_2.ref t (Root 0)
+
+let rec repr t elt =
+  match Pstore_2.get t elt with
+  | Root _ ->
+      elt
+  | Link parent ->
+      let repr = repr t parent in
+      Pstore_2.set t elt (Link repr) ;
+      repr
+
+let equiv t elt1 elt2 =
+  repr t elt1 == repr t elt2
+
+let[@inline] rank t elt =
+  match Pstore_2.get t elt with
+  | Root rank ->
+      rank
+  | Link _ ->
+      assert false
+let union t elt1 elt2 =
+  let repr1 = repr t elt1 in
+  let rank1 = rank t repr1 in
+  let repr2 = repr t elt2 in
+  let rank2 = rank t repr2 in
+  if repr1 != repr2 then
+    if rank1 < rank2 then (
+      Pstore_2.set t repr1 (Link repr2)
+    ) else (
+      Pstore_2.set t repr2 (Link repr1) ;
+      if rank1 == rank2 then
+        Pstore_2.set t repr1 (Root (rank1 + 1))
+    )
+
+type snapshot =
+  descr Pstore_2.snapshot
+
+let capture =
+  Pstore_2.capture
+
+let restore =
+  Pstore_2.restore
