lib/zoo_persistent/puf.mli
@@ -1,0 +1,26 @@
+type element
+
+type t
+
+val create :
+  unit -> t
+
+val make :
+  t -> element
+
+val repr :
+  t -> element -> element
+
+val equiv :
+  t -> element -> element -> bool
+
+val union :
+  t -> element -> element -> unit
+
+type snapshot
+
+val capture :
+  t -> snapshot
+
+val restore :
+  t -> snapshot -> unit
