theories/zoo_persistent/puf.v
@@ -1,0 +1,507 @@
+From zoo Require Import
+  prelude.
+From zoo.common Require Import
+  fin_maps.
+From zoo.language Require Import
+  notations.
+From zoo.diaframe Require Import
+  diaframe.
+From zoo_persistent Require Export
+  base
+  puf__code.
+From zoo_persistent Require Import
+  puf__types
+  pstore_2.
+From zoo Require Import
+  options.
+
+Implicit Types rank : Z.
+Implicit Types elt repr parent : location.
+Implicit Types t s descr : val.
+Implicit Types reprs : gmap location location.
+Implicit Types descrs : gmap location val.
+
+Class PufG Σ `{zoo_G : !ZooG Σ} := {
+  #[local] puf_G_pstore_G :: Pstore2G Σ ;
+}.
+
+Definition puf_Σ := #[
+  pstore_2_Σ
+].
+#[global] Instance subG_puf_Σ Σ `{zoo_G : !ZooG Σ} :
+  subG puf_Σ Σ →
+  PufG Σ.
+Proof.
+  solve_inG.
+Qed.
+
+Section puf_G.
+  Context `{puf_G : PufG Σ}.
+
+  #[local] Definition consistent_at reprs elt repr descr :=
+    ( ∃ rank,
+      repr = elt ∧
+      descr = ‘Root( #rank )%V
+    ) ∨ (
+      ∃ parent,
+      elt ≠ repr ∧
+      descr = ‘Link( #parent )%V ∧
+      reprs !! parent = Some repr ∧
+      reprs !! repr = Some repr
+    ).
+  #[local] Definition consistent reprs descrs :=
+    map_Forall2 (consistent_at reprs) reprs descrs.
+
+  Definition puf_model t reprs : iProp Σ :=
+    ∃ descrs,
+    pstore_2_model t descrs ∗
+    ⌜consistent reprs descrs⌝.
+  #[local] Instance : CustomIpatFormat "model" :=
+    "(
+      %descrs{} &
+      Hmodel{} &
+      %Hconsistent{}
+    )".
+
+  Definition puf_snapshot s t reprs : iProp Σ :=
+    ∃ descrs,
+    pstore_2_snapshot s t descrs ∗
+    ⌜consistent reprs descrs⌝.
+  #[local] Instance : CustomIpatFormat "snapshot" :=
+    "(
+      %descrs{} &
+      Hsnapshot{} &
+      %Hconsistent{}
+    )".
+
+  #[global] Instance puf_model_timeless t reprs :
+    Timeless (puf_model t reprs).
+  Proof.
+    apply _.
+  Qed.
+  #[global] Instance puf_snapshot_persistent s t reprs :
+    Persistent (puf_snapshot s t reprs).
+  Proof.
+    apply _.
+  Qed.
+
+  #[local] Definition unify_at repr1 repr2 repr :=
+    if decide (repr = repr1) then
+      repr2
+    else
+      repr.
+
+  #[local] Lemma unify_at_1 repr1 repr2 :
+    unify_at repr1 repr2 repr1 = repr2.
+  Proof.
+    rewrite /unify_at decide_True //.
+  Qed.
+  #[local] Lemma unify_at_2 repr1 repr2 repr :
+    repr ≠ repr1 →
+    unify_at repr1 repr2 repr = repr.
+  Proof.
+    intros.
+    rewrite /unify_at decide_False //.
+  Qed.
+
+  #[local] Definition unify repr1 repr2 reprs :=
+    unify_at repr1 repr2 <$> reprs.
+
+  #[local] Lemma unify_lookup_1 reprs repr1 repr2 elt :
+    reprs !! elt = Some repr1 →
+    unify repr1 repr2 reprs !! elt = Some repr2.
+  Proof.
+    intros Hreprs_lookup_elt.
+    rewrite lookup_fmap Hreprs_lookup_elt /= unify_at_1 //.
+  Qed.
+  #[local] Lemma unify_lookup_2 {reprs repr1 repr2 elt} repr :
+    reprs !! elt = Some repr →
+    repr ≠ repr1 →
+    unify repr1 repr2 reprs !! elt = Some repr.
+  Proof.
+    intros Hreprs_lookup_elt ?.
+    rewrite lookup_fmap Hreprs_lookup_elt /= unify_at_2 //.
+  Qed.
+  #[local] Lemma unify_lookup_2' reprs repr1 repr2 :
+    reprs !! repr2 = Some repr2 →
+    repr1 ≠ repr2 →
+    unify repr1 repr2 reprs !! repr2 = Some repr2.
+  Proof.
+    intros.
+    apply unify_lookup_2; done.
+  Qed.
+
+  #[local] Lemma consistent_lookup_None {reprs descrs} elt :
+    consistent reprs descrs →
+    descrs !! elt = None →
+    reprs !! elt = None.
+  Proof.
+    apply: map_Forall2_lookup_None_r.
+  Qed.
+  #[local] Lemma consistent_lookup_Some {reprs descrs} elt repr :
+    consistent reprs descrs →
+    reprs !! elt = Some repr →
+      ∃ descr,
+      descrs !! elt = Some descr ∧
+      consistent_at reprs elt repr descr.
+  Proof.
+    apply: map_Forall2_lookup_Some_l.
+  Qed.
+  #[local] Lemma consistent_insert {reprs descrs} elt :
+    descrs !! elt = None →
+    consistent reprs descrs →
+    consistent
+      (<[elt := elt]> reprs)
+      (<[elt := ‘Root( #0 )%V]> descrs).
+  Proof.
+    rewrite /consistent /consistent_at.
+    intros Hdescrs_lookup Hconsistent.
+    eapply consistent_lookup_None in Hconsistent as Hresprs_lookup; last done.
+    apply map_Forall2_insert_2; first naive_solver.
+    eapply map_Forall2_impl; first done.
+    intros elt' repr' descr' [| (parent & ? & -> & Hreprs_lookup_parent & Hreprs_lookup_repr)]; first auto.
+    right. exists parent.
+    rewrite !lookup_insert_ne //; congruence.
+  Qed.
+  #[local] Lemma consistent_link_repr {reprs descrs} elt repr :
+    elt ≠ repr →
+    reprs !! elt = Some repr →
+    reprs !! repr = Some repr →
+    consistent reprs descrs →
+    consistent
+      reprs
+      (<[elt := ‘Link( #repr )%V]> descrs).
+  Proof.
+    rewrite /consistent.
+    intros ? Hreprs_lookup_elt Hreprs_lookup_repr Hconsistent.
+    eapply map_Forall2_insert_r; [done.. |].
+    right. eauto.
+  Qed.
+  #[local] Lemma consistent_link_union {reprs descrs} repr1 repr2 :
+    repr1 ≠ repr2 →
+    reprs !! repr1 = Some repr1 →
+    reprs !! repr2 = Some repr2 →
+    consistent reprs descrs →
+    consistent
+      (unify repr1 repr2 reprs)
+      (<[repr1 := ‘Link( #repr2 )%V]> descrs).
+  Proof.
+    rewrite /consistent.
+    intros ? Hreprs_lookup_repr1 Hreprs_lookup_repr2 Hconsistent.
+    apply map_Forall2_alt in Hconsistent as (Hdom & Hconsistent).
+    rewrite -map_Forall2_fmap_l map_Forall2_alt.
+    split.
+    - apply elem_of_dom_2 in Hreprs_lookup_repr1.
+      set_solver.
+    - intros elt repr descr Hreprs_lookup_elt [(<- & <-) | (? & Hdescrs_lookup_elt)]%lookup_insert_Some. simplify.
+      + right. exists repr2.
+        rewrite unify_at_1 unify_lookup_2' //.
+      + destruct (decide (repr = repr1)) as [-> |].
+        * rewrite unify_at_1.
+          ospecialize* (Hconsistent elt); [done.. |].
+          destruct Hconsistent as [| (parent & ? & -> & Hreprs_lookup_parent & Hreprs_lookup_repr1_)]; first naive_solver. simplify.
+          right. exists parent.
+          rewrite unify_lookup_1 // unify_lookup_2' //.
+          naive_solver.
+        * rewrite unify_at_2 //.
+          ospecialize* (Hconsistent elt); [done.. |].
+          destruct Hconsistent as [(rank & <- & ->)| (parent & ? & -> & Hreprs_lookup_parent & Hreprs_lookup_repr1_)].
+          -- left. naive_solver.
+          -- right. exists parent.
+             rewrite !(unify_lookup_2 repr) //.
+  Qed.
+  #[local] Lemma consistent_update_rank {reprs descrs} repr rank :
+    reprs !! repr = Some repr →
+    consistent reprs descrs →
+    consistent
+      reprs
+      (<[repr := ‘Root( #rank )%V]> descrs).
+  Proof.
+    rewrite /consistent.
+    intros Hreprs_lookup_repr Hconsistent.
+    eapply map_Forall2_insert_r; [done.. |].
+    left. eauto.
+  Qed.
+
+  Lemma puf_model_valid {t reprs} elt repr :
+    reprs !! elt = Some repr →
+    puf_model t reprs ⊢
+    ⌜reprs !! repr = Some repr⌝.
+  Proof.
+    iIntros "%Hreprs_lookup (:model)". iPureIntro.
+    eapply consistent_lookup_Some in Hconsistent as (descr & Hdescrs_lookup & []); last done.
+    all: naive_solver.
+  Qed.
+  Lemma puf_model_exclusive t reprs1 reprs2 :
+    puf_model t reprs1 -∗
+    puf_model t reprs2 -∗
+    False.
+  Proof.
+    iIntros "(:model =1) (:model =2)".
+    iApply (pstore_2_model_exclusive with "Hmodel1 Hmodel2").
+  Qed.
+
+  Lemma puf_create_spec :
+    {{{
+      True
+    }}}
+      puf_create ()
+    {{{ t,
+      RET t;
+      puf_model t ∅
+    }}}.
+  Proof.
+    iIntros "%Φ _ HΦ".
+
+    wp_apply (pstore_2_create_spec with "[//]").
+    iSteps.
+  Qed.
+
+  Lemma puf_make_spec t reprs :
+    {{{
+      puf_model t reprs
+    }}}
+      puf_make t
+    {{{ elt,
+      RET #elt;
+      puf_model t (<[elt := elt]> reprs)
+    }}}.
+  Proof.
+    iIntros "%Φ (:model) HΦ".
+
+    wp_rec.
+    wp_smart_apply (pstore_2_ref_spec with "Hmodel") as (elt) "(%Hdescrs_lookup & Hmodel)".
+
+    eapply consistent_insert in Hconsistent; last done.
+    iSteps.
+  Qed.
+
+  #[local] Lemma puf_repr_spec {t reprs elt} repr :
+    reprs !! elt = Some repr →
+    {{{
+      puf_model t reprs
+    }}}
+      puf_repr t #elt
+    {{{
+      RET #repr;
+      puf_model t reprs
+    }}}.
+  Proof.
+    iLöb as "HLöb" forall (elt repr).
+
+    iIntros "%Hreprs_lookup_elt %Φ (:model) HΦ".
+    pose proof Hconsistent as (descr & Hdescrs_lookup & Hconsistent_at)%(consistent_lookup_Some elt repr); last done.
+
+    wp_rec.
+    wp_smart_apply (pstore_2_get_spec with "Hmodel") as "Hmodel"; first done.
+
+    destruct Hconsistent_at as [(rank & -> & ->) | (parent & ? & -> & Hreprs_lookup_parent & Hreprs_lookup_repr)]; wp_pures; first iSteps.
+
+    wp_apply ("HLöb" $! parent with "[//] [$Hmodel //]") as "(:model =')".
+    pose proof Hconsistent' as (descr' & Hdescrs'_lookup & _)%(consistent_lookup_Some elt repr); last done.
+
+    wp_smart_apply (pstore_2_set_spec with "Hmodel'") as "Hmodel".
+    { rewrite elem_of_dom //. }
+    wp_pures.
+
+    apply (consistent_link_repr elt repr) in Hconsistent'; [| done..].
+    iSteps.
+  Qed.
+
+  Lemma puf_equiv_spec {t reprs elt1} repr1 {elt2} repr2 :
+    reprs !! elt1 = Some repr1 →
+    reprs !! elt2 = Some repr2 →
+    {{{
+      puf_model t reprs
+    }}}
+      puf_equiv t #elt1 #elt2
+    {{{
+      RET #(bool_decide (repr1 = repr2));
+      puf_model t reprs
+    }}}.
+  Proof.
+    iIntros "%Hreprs_lookup_elt1 %Hreprs_lookup_elt2 %Φ Hmodel HΦ".
+
+    wp_rec.
+    wp_smart_apply (puf_repr_spec with "Hmodel") as "Hmodel"; first done.
+    wp_smart_apply (puf_repr_spec with "Hmodel") as "Hmodel"; first done.
+    iSteps.
+  Qed.
+
+  #[local] Lemma puf_rank_spec t reprs elt :
+    reprs !! elt = Some elt →
+    {{{
+      puf_model t reprs
+    }}}
+      puf_rank t #elt
+    {{{ rank,
+      RET #rank;
+      puf_model t reprs
+    }}}.
+  Proof.
+    iIntros "%Hreprs_lookup_elt %Φ (:model) HΦ".
+    pose proof Hconsistent as (descr & Hdescrs_lookup & Hconsistent_at)%(consistent_lookup_Some elt elt); last done.
+
+    wp_rec.
+    wp_smart_apply (pstore_2_get_spec with "Hmodel") as "Hmodel"; first done.
+
+    destruct Hconsistent_at as [(rank & _ & ->) | (parent & ? & -> & Hreprs_lookup_parent & Hreprs_lookup_repr)]; last done.
+    iSteps.
+  Qed.
+  Definition puf_union_condition reprs repr1 repr2 reprs' :=
+    dom reprs = dom reprs' ∧
+    ( ∀ elt repr,
+      reprs !! elt = Some repr →
+      repr ≠ repr1 →
+      repr ≠ repr2 →
+      reprs' !! elt = Some repr
+    ) ∧
+    ( ∃ repr12,
+      (repr12 = repr1 ∨ repr12 = repr2) ∧
+        ∀ elt repr,
+        reprs !! elt = Some repr →
+        repr = repr1 ∨ repr = repr2 →
+        reprs' !! elt = Some repr12
+    ).
+  #[local] Lemma puf_union_condition_refl reprs repr :
+    puf_union_condition reprs repr repr reprs.
+  Proof.
+    split_and!; [done.. |].
+    naive_solver.
+  Qed.
+  #[local] Lemma puf_union_condition_sym reprs repr1 repr2 reprs' :
+    puf_union_condition reprs repr1 repr2 reprs' →
+    puf_union_condition reprs repr2 repr1 reprs'.
+  Proof.
+    rewrite /puf_union_condition.
+    intros (Hdom & Hunchanged & (repr12 & Hchanged)).
+    split_and!; auto.
+    exists repr12. naive_solver.
+  Qed.
+  #[local] Lemma unify_union_condition_1 reprs repr1 repr2 :
+    repr1 ≠ repr2 →
+    puf_union_condition reprs repr1 repr2 (unify repr1 repr2 reprs).
+  Proof.
+    intros.
+    split_and!.
+    - set_solver.
+    - intros.
+      apply unify_lookup_2; done.
+    - exists repr2. split; first auto.
+      intros elt repr Hreprs_lookup_elt [-> | ->].
+      + rewrite unify_lookup_1 //.
+      + rewrite (unify_lookup_2 repr2) //.
+  Qed.
+  #[local] Lemma unify_union_condition_2 reprs repr1 repr2 :
+    repr1 ≠ repr2 →
+    puf_union_condition reprs repr2 repr1 (unify repr1 repr2 reprs).
+  Proof.
+    intros.
+    apply puf_union_condition_sym, unify_union_condition_1; done.
+  Qed.
+  #[local] Opaque puf_union_condition.
+  Lemma puf_union_spec {t reprs elt1} repr1 {elt2} repr2 :
+    reprs !! elt1 = Some repr1 →
+    reprs !! elt2 = Some repr2 →
+    {{{
+      puf_model t reprs
+    }}}
+      puf_union t #elt1 #elt2
+    {{{ reprs',
+      RET ();
+      puf_model t reprs' ∗
+      ⌜puf_union_condition reprs repr1 repr2 reprs'⌝
+    }}}.
+  Proof.
+    iIntros "%Hreprs_lookup_elt1 %Hreprs_lookup_elt2 %Φ Hmodel HΦ".
+    iDestruct (puf_model_valid elt1 with "Hmodel") as %Hreprs_lookup_repr1; first done.
+    iDestruct (puf_model_valid elt2 with "Hmodel") as %Hreprs_lookup_repr2; first done.
+
+    wp_rec.
+    wp_smart_apply (puf_repr_spec with "Hmodel") as "Hmodel"; first done.
+    wp_smart_apply (puf_rank_spec with "Hmodel") as (rank1) "Hmodel"; first done.
+    wp_smart_apply (puf_repr_spec with "Hmodel") as "Hmodel"; first done.
+    wp_smart_apply (puf_rank_spec with "Hmodel") as (rank2) "(:model)"; first done.
+
+    pose proof Hconsistent as (descr1 & Hdescrs_lookup_1 & Hconsistent_at_1)%(consistent_lookup_Some repr1 repr1); last done.
+    pose proof Hconsistent as (descr2 & Hdescrs_lookup_2 & Hconsistent_at_2)%(consistent_lookup_Some repr2 repr2); last done.
+
+    wp_pures.
+    case_bool_decide; first subst repr2.
+
+    - iSteps. iPureIntro. apply puf_union_condition_refl.
+
+    - wp_pures.
+      case_bool_decide; wp_pures.
+
+      + wp_apply (pstore_2_set_spec with "Hmodel") as "Hmodel".
+        { rewrite elem_of_dom //. }
+        apply (consistent_link_union repr1 repr2) in Hconsistent; [| done..].
+
+        iApply ("HΦ" $! (unify repr1 repr2 reprs)).
+        iSteps. iPureIntro. apply unify_union_condition_1. done.
+
+      + wp_apply (pstore_2_set_spec with "Hmodel") as "Hmodel".
+        { rewrite elem_of_dom //. }
+        apply (consistent_link_union repr2 repr1) in Hconsistent; [| done..].
+
+        wp_pures.
+        case_bool_decide; wp_pures.
+
+        * wp_apply (pstore_2_set_spec with "Hmodel") as "Hmodel".
+          { apply dom_insert, elem_of_union_r, elem_of_dom. done. }
+          eapply (consistent_update_rank repr1) in Hconsistent; last first.
+          { rewrite unify_lookup_2' //. }
+
+          iApply ("HΦ" $! (unify repr2 repr1 reprs)).
+          iSteps. iPureIntro. apply unify_union_condition_2. done.
+
+        * iApply ("HΦ" $! (unify repr2 repr1 reprs)).
+          iSteps. iPureIntro. apply unify_union_condition_2. done.
+  Qed.
+
+  Lemma puf_capture_spec t reprs :
+    {{{
+      puf_model t reprs
+    }}}
+      puf_capture t
+    {{{ s,
+      RET s;
+      puf_model t reprs ∗
+      puf_snapshot s t reprs
+    }}}.
+  Proof.
+    iIntros "%Φ (:model) HΦ".
+
+    wp_apply (pstore_2_capture_spec with "Hmodel").
+    iSteps.
+  Qed.
+
+  Lemma puf_restore_spec t reprs s reprs' :
+    {{{
+      puf_model t reprs ∗
+      puf_snapshot s t reprs'
+    }}}
+      puf_restore t s
+    {{{ s,
+      RET s;
+      puf_model t reprs'
+    }}}.
+  Proof.
+    iIntros "%Φ ((:model) & (:snapshot =')) HΦ".
+
+    wp_apply (pstore_2_restore_spec with "[$Hmodel $Hsnapshot']").
+    iSteps.
+  Qed.
+End puf_G.
+
+#[global] Opaque puf_create.
+#[global] Opaque puf_make.
+#[global] Opaque puf_repr.
+#[global] Opaque puf_equiv.
+#[global] Opaque puf_union.
+#[global] Opaque puf_capture.
+#[global] Opaque puf_restore.
+
+#[global] Opaque puf_model.
+#[global] Opaque puf_snapshot.
