theories/zoo_persistent/puf__code.v
@@ -1,0 +1,65 @@
+From zoo Require Import
+  prelude.
+From zoo.language Require Import
+  typeclasses
+  notations.
+From zoo_persistent Require Import
+  pstore_2.
+From zoo_persistent Require Import
+  puf__types.
+From zoo Require Import
+  options.
+
+Definition puf_create : val :=
+  pstore_2_create.
+
+Definition puf_make : val :=
+  fun: "t" =>
+    pstore_2_ref "t" ‘Root( #0 ).
+
+Definition puf_repr : val :=
+  rec: "repr" "t" "elt" =>
+    match: pstore_2_get "t" "elt" with
+    | Root <> =>
+        "elt"
+    | Link "parent" =>
+        let: "repr" := "repr" "t" "parent" in
+        pstore_2_set "t" "elt" ‘Link( "repr" ) ;;
+        "repr"
+    end.
+
+Definition puf_equiv : val :=
+  fun: "t" "elt1" "elt2" =>
+    puf_repr "t" "elt1" == puf_repr "t" "elt2".
+
+Definition puf_rank : val :=
+  fun: "t" "elt" =>
+    match: pstore_2_get "t" "elt" with
+    | Root "rank" =>
+        "rank"
+    | Link <> =>
+        Fail
+    end.
+
+Definition puf_union : val :=
+  fun: "t" "elt1" "elt2" =>
+    let: "repr1" := puf_repr "t" "elt1" in
+    let: "rank1" := puf_rank "t" "repr1" in
+    let: "repr2" := puf_repr "t" "elt2" in
+    let: "rank2" := puf_rank "t" "repr2" in
+    if: "repr1" != "repr2" then (
+      if: "rank1" < "rank2" then (
+        pstore_2_set "t" "repr1" ‘Link( "repr2" )
+      ) else (
+        pstore_2_set "t" "repr2" ‘Link( "repr1" ) ;;
+        if: "rank1" == "rank2" then (
+          pstore_2_set "t" "repr1" ‘Root( "rank1" + #1 )
+        )
+      )
+    ).
+
+Definition puf_capture : val :=
+  pstore_2_capture.
+
+Definition puf_restore : val :=
+  pstore_2_restore.
