theories/zoo_persistent/puf__types.v
@@ -1,0 +1,18 @@
+From zoo Require Import
+  prelude.
+From zoo.language Require Import
+  typeclasses
+  notations.
+From zoo_persistent Require Import
+  pstore_2.
+From zoo Require Import
+  options.
+
+Notation "'Root'" := (
+  in_type "zoo_persistent.puf.descr" 0
+)(in custom zoo_tag
+).
+Notation "'Link'" := (
+  in_type "zoo_persistent.puf.descr" 1
+)(in custom zoo_tag
+).
